imp/Imp/Hoare.lean
@@ -1,2 +1,3 @@
 import Imp.Hoare.Basic
+import Imp.Hoare.Syntax
 import Imp.Hoare.Rules
