imp/Imp/Hoare/Basic.lean
@@ -2,55 +2,98 @@ import Imp.Expr.Eval
 import Imp.Stmt.BigStep
 import Imp.Stmt.Basic
 
-open Imp Stmt
+open Imp
 
 def Assertion : Type := Env → Prop
+syntax "{{ " term:50 " }}" : term
+macro_rules
+  | `({{ $P }}) => `(($P : Assertion))
 
 @[simp]
 def ValidHoareTriple (P : Assertion) (c : Stmt) (Q : Assertion) : Prop :=
   forall (σ σ' : Env), P σ -> c / σ ↓ σ' -> Q σ'
 
-syntax "{{" term:90 "}} " term:91 " {{" term:92 "}}" : term
+syntax "{{" term:60 "}} " term:61 " {{" term:62 "}}" : term
 macro_rules
   | `({{ $P }} $c{{ $Q }}) => `(ValidHoareTriple $P $c $Q)
 
+namespace Assertion
+
 @[simp]
-def Assertion.implies (P Q : Assertion) : Prop :=
+def implies (P Q : Assertion) : Prop :=
   forall σ, P σ → Q σ
 syntax term:90 "->>" term:91 : term
 macro_rules
-  | `($P ->> $Q) => `(Assertion.implies $P $Q)
+  | `($P ->> $Q) => `(implies $P $Q)
 
 @[simp]
-def Assertion.iff (P Q : Assertion) : Prop :=
+def iff (P Q : Assertion) : Prop :=
   forall σ, P σ ↔ Q σ
 syntax term:90 "<<->>" term:91 : term
 macro_rules
-  | `($P <<->> $Q) => `(Assertion.iff $P $Q)
+  | `($P <<->> $Q) => `(iff $P $Q)
 
 @[simp]
-def Assertion.substitution (P : Assertion) (x : String) (a : Expr) : Assertion :=
+def substitution (P : Assertion) (x : String) (a : Expr) : Assertion :=
   fun σ => P (σ.setOption x (a.eval σ))
 syntax term " [ " ident " ↦ " term "]" : term
 macro_rules
-  | `($P [$x ↦ $a]) => `(Assertion.substitution $P $x $a)
+  | `($P [$x ↦ $a]) => `(substitution $P $x $a)
+
+@[simp]
+def and (P Q : Assertion) : Assertion :=
+  fun σ => P σ ∧ Q σ
+syntax term:90 " <^> " term:91 : term
+macro_rules
+  | `($P <^> $Q) => `(and $P $Q)
+
+@[simp]
+def not (P : Assertion) : Assertion :=
+  fun σ => ¬ P σ
+macro_rules
+  | `(! $P) => `(not $P)
+
+end Assertion
 
 instance : Coe Expr Assertion where
   coe b := fun σ => Truthy $ b.eval σ
-
-@[simp]
-def Assertion.and (P Q : Assertion) : Assertion :=
-  fun σ => P σ ∧ Q σ
-macro_rules
-  | `($P ∧ $Q) => `(Assertion.and $P $Q)
-
-@[simp]
-def Assertion.not (P : Assertion) : Assertion :=
-  fun σ => ¬ P σ
-macro_rules
-  | `(! $P) => `(Assertion.not $P)
-
 @[simp]
 theorem Truthy.assert_true : ∀ (b : Expr), (fun σ => Truthy (b.eval σ)) <<->> b := by
   intro b σ
   constructor <;> intro h <;> assumption
+
+instance ExprToBool (σ : Env) : Coe Expr Bool where
+  coe b := Truthy $ b.eval σ
+instance ExprToValue (σ : Env) : Coe Expr Prop where
+  coe b := Truthy $ b.eval σ
+
+instance : Coe Prop Assertion where
+  coe P := fun _ => P
+instance : Coe Bool Assertion where
+  coe b := fun _ => if b then True else False
+
+-- def Assertion.expInt : Type := Env → Int
+-- def Assertion.expV : Type := Env -> Value
+-- instance : Coe Int Assertion.expInt where
+--   coe i := fun _ => i
+-- instance : Coe Value Assertion.expInt where
+--   coe v := fun _ => v
+-- instance : Coe Value Assertion.expV where
+--   coe v := fun _ => v
+-- instance : Coe Expr Assertion.expInt where
+--   coe e := fun σ => match e.eval σ with
+--     | some i => i
+--     | none => 0
+-- instance : Coe Expr Assertion.expV where
+--   coe e := fun σ => match e.eval σ with
+--     | some v => v
+--     | none => Value.int 0
+--
+-- instance : Coe String Assertion.expInt where
+--   coe s := fun σ => σ s
+-- instance : Coe String Assertion.expV where
+--   coe s := fun σ => σ s
+-- instance expIntToExpr (σ : Env) : Coe Assertion.expInt Expr where
+--   coe i := Expr.const $ i σ
+-- instance ExpVToExpr (σ : Env) : Coe Assertion.expV Expr where
+--   coe v := Expr.const $ v σ
