imp/Imp/Hoare/Syntax.lean
@@ -1,0 +1,148 @@
+import Lean
+import Imp.Hoare.Basic
+
+open Lean Elab Meta
+
+declare_syntax_cat assertion
+syntax ident "=" num : assertion
+syntax num "=" ident : assertion
+syntax ident "=" ident : assertion
+syntax ident "!=" num : assertion
+syntax num "!=" ident : assertion
+syntax ident "!=" ident : assertion
+syntax ident "<" num : assertion
+syntax num "<" ident : assertion
+syntax ident "<" ident : assertion
+syntax ident ">" num : assertion
+syntax num ">" ident : assertion
+syntax ident ">" ident : assertion
+syntax ident "<=" num : assertion
+syntax num "<=" ident : assertion
+syntax ident "<=" ident : assertion
+syntax ident ">=" num : assertion
+syntax num ">=" ident : assertion
+syntax ident ">=" ident : assertion
+syntax assertion " <^> " assertion : assertion
+syntax "!" assertion : assertion
+syntax assertion " ->> " assertion : assertion
+syntax assertion " <<->> " assertion : assertion
+
+@[simp] def strValEq (x : String) (n : Int) : Assertion := fun σ => σ x = n
+@[simp] def strValNe (x : String) (n : Int) : Assertion := fun σ => σ x ≠ n
+@[simp] def strValLt (x : String) (n : Int) : Assertion := fun σ => σ x < n
+@[simp] def strValGt (x : String) (n : Int) : Assertion := fun σ => σ x > n
+@[simp] def strValLe (x : String) (n : Int) : Assertion := fun σ => σ x ≤ n
+@[simp] def strValGe (x : String) (n : Int) : Assertion := fun σ => σ x ≥ n
+@[simp] def strStrEq (x y : String) : Assertion := fun σ => σ x = σ y
+@[simp] def strStrNe (x y : String) : Assertion := fun σ => σ x ≠ σ y
+@[simp] def strStrLt (x y : String) : Assertion := fun σ => σ x < σ y
+@[simp] def strStrGt (x y : String) : Assertion := fun σ => σ x > σ y
+@[simp] def strStrLe (x y : String) : Assertion := fun σ => σ x ≤ σ y
+@[simp] def strStrGe (x y : String) : Assertion := fun σ => σ x ≥ σ y
+partial def elabAssertionLit : Syntax → MetaM Expr
+  -- Eq
+  | `(assertion| $x:ident = $n:num) => do
+    let x <- pure $ mkStrLit x.getId.toString
+    let n <- pure $ mkIntLit n.getNat
+    mkAppM ``strValEq  #[x, n]
+  | `(assertion| $n:num = $x:ident) => do
+    let x <- pure $ mkStrLit x.getId.toString
+    let n <- pure $ mkIntLit n.getNat
+    mkAppM ``strValEq  #[x, n]
+  | `(assertion| $x:ident = $y:ident) => do
+    let x <- pure $ mkStrLit x.getId.toString
+    let y <- pure $ mkStrLit y.getId.toString
+    mkAppM ``strStrEq  #[x, y]
+  -- Neq
+  | `(assertion| $x:ident != $n:num) => do
+    let x <- pure $ mkStrLit x.getId.toString
+    let n <- pure $ mkIntLit n.getNat
+    mkAppM ``strValNe  #[x, n]
+  | `(assertion| $n:num != $x:ident) => do
+    let x <- pure $ mkStrLit x.getId.toString
+    let n <- pure $ mkIntLit n.getNat
+    mkAppM ``strValNe  #[x, n]
+  | `(assertion| $x:ident != $y:ident) => do
+    let x <- pure $ mkStrLit x.getId.toString
+    let y <- pure $ mkStrLit y.getId.toString
+    mkAppM ``strStrNe  #[x, y]
+  -- LT
+  | `(assertion| $x:ident < $n:num) => do
+    let x <- pure $ mkStrLit x.getId.toString
+    let n <- pure $ mkIntLit n.getNat
+    mkAppM ``strValLt  #[x, n]
+  | `(assertion| $n:num < $x:ident) => do
+    let x <- pure $ mkStrLit x.getId.toString
+    let n <- pure $ mkIntLit n.getNat
+    mkAppM ``strValLt  #[x, n]
+  | `(assertion| $x:ident < $y:ident) => do
+    let x <- pure $ mkStrLit x.getId.toString
+    let y <- pure $ mkStrLit y.getId.toString
+    mkAppM ``strStrLt  #[x, y]
+  -- GT
+  | `(assertion| $x:ident > $n:num) => do
+    let x <- pure $ mkStrLit x.getId.toString
+    let n <- pure $ mkIntLit n.getNat
+    mkAppM ``strValGt  #[x, n]
+  | `(assertion| $n:num > $x:ident) => do
+    let x <- pure $ mkStrLit x.getId.toString
+    let n <- pure $ mkIntLit n.getNat
+    mkAppM ``strValGt  #[x, n]
+  |`(assertion| $x:ident > $y:ident) => do
+    let x <- pure $ mkStrLit x.getId.toString
+    let y <- pure $ mkStrLit y.getId.toString
+    mkAppM ``strStrGt  #[x, y]
+  -- LE
+  | `(assertion| $x:ident <= $n:num) => do
+    let x <- pure $ mkStrLit x.getId.toString
+    let n <- pure $ mkIntLit n.getNat
+    mkAppM ``strValLe  #[x, n]
+  | `(assertion| $n:num <= $x:ident) => do
+    let x <- pure $ mkStrLit x.getId.toString
+    let n <- pure $ mkIntLit n.getNat
+    mkAppM ``strValLe  #[x, n]
+  | `(assertion| $x:ident <= $y:ident) => do
+    let x <- pure $ mkStrLit x.getId.toString
+    let y <- pure $ mkStrLit y.getId.toString
+    mkAppM ``strStrLe  #[x, y]
+  -- GE
+  | `(assertion| $x:ident >= $n:num) => do
+    let x <- pure $ mkStrLit x.getId.toString
+    let n <- pure $ mkIntLit n.getNat
+    mkAppM ``strValGe  #[x, n]
+  | `(assertion| $n:num >= $x:ident) => do
+    let x <- pure $ mkStrLit x.getId.toString
+    let n <- pure $ mkIntLit n.getNat
+    mkAppM ``strValGe  #[x, n]
+  | `(assertion| $x:ident >= $y:ident) => do
+    let x <- pure $ mkStrLit x.getId.toString
+    let y <- pure $ mkStrLit y.getId.toString
+    mkAppM ``strStrGe  #[x, y]
+  -- Conjunction
+  | `(assertion| $a:assertion <^> $b:assertion) => do
+        let a <- elabAssertionLit a
+        let b <- elabAssertionLit b
+        mkAppM ``Assertion.and #[a, b]
+  -- Negation
+  | `(assertion| ! $a:assertion) => do
+        let a <- elabAssertionLit a
+        mkAppM ``Assertion.not #[a]
+  -- Implication
+  | `(assertion| $a:assertion ->> $b:assertion) => do
+        let a <- elabAssertionLit a
+        let b <- elabAssertionLit b
+        mkAppM ``Assertion.implies #[a, b]
+  -- Biimplication
+  | `(assertion| $a:assertion <<->> $b:assertion) => do
+        let a <- elabAssertionLit a
+        let b <- elabAssertionLit b
+        mkAppM ``Assertion.iff #[a, b]
+  | _ => throwUnsupportedSyntax
+
+elab "astn " a:assertion : term => elabAssertionLit a
+
+/--
+info: (strStrLe "y" "z").and (strValGt "x" 5) : Assertion
+-/
+#guard_msgs in
+#check astn y <= z <^> x > 5
